\section*{The Homotopy Axiom}
\subsection*{The Acyclic Models Theorem}

\begin{proposition}
	Let $\mathcal{C}$ be a locally small category with family of models $(M_\alpha)_{\alpha \in A}$ and $K,L : \mathcal{C} \to \mathsf{AbGrp}$ two functors, where $L$ is free with basis in $(M_\alpha)_{\alpha \in A}$ and model basis $(g_\alpha)_{\alpha \in A}$ for $L$. Moreover, let $(h_\alpha)_{\alpha \in A}$ be a family such that $h_\alpha \in K(M_\alpha)$ for all $\alpha \in A$. Then there exists a uniqe natural transformation $\Phi : L \Rightarrow K$ such that $\Phi_{M_\alpha}(g_\alpha) = h_\alpha$ for all $\alpha \in A$.
\end{proposition}



\subsection*{Chain Homotopies and the Homotopy Axiom}
\begin{definition}[Chain Homotopies]
	Two chain maps $f_\bullet,g_\bullet : (C_\bullet,\partial_\bullet) \to (C_\bullet',\partial_\bullet')$ are said to be \bld{chain homotopic}, written $f_\bullet \simeq g_\bullet$, if there exists a sequence $(F_n)_{n \in \mathbb{Z}}$, such that $F_n \in \mathsf{AbGrp}(C_n,C_{n + 1}')$ and 
	\begin{equation*}
		\partial_{n + 1}' \circ F_n + F_{n - 1} \circ \partial_n = f_n - g_n,
	\end{equation*}
	\noindent for all $n \in \mathbb{Z}$. The sequence $(F_n)_{n \in \mathbb{Z}}$ is then called a \bld{chain homotopy} and is written $F : f_\bullet \simeq g_\bullet$.
\end{definition}

\begin{proposition}
	\label{prop:inclusions}
	Let $f_\bullet,g_\bullet \in \mathsf{Comp}(C_\bullet,C_\bullet')$ with $f \simeq g$. Then $H_n(f_\bullet) = H_n(g_\bullet)$ for all $n \in \mathbb{Z}$.
\end{proposition}

\begin{proof}
	Assume $F : f_\bullet \simeq g_\bullet$ and let $\langle c \rangle \in H_n(C_\bullet) \to H_n(C_\bullet')$. Then
	\begin{align*}
		H_n(f_\bullet)\langle c \rangle &= \langle f_n(c) \rangle\\
		&= \langle g_n(c) + \partial_{n + 1}'(F_n(c)) + F_{n - 1}(\partial_n(c)) \rangle\\
		&= \langle g_n(c) + \partial_{n + 1}'(F_n(c)) \rangle\\
		&= \langle g_n(c) \rangle\\
		&= H_n(g_\bullet)\langle c \rangle
	\end{align*}
	\noindent since $c \in \ker \partial_n$.
\end{proof}

\begin{proposition}
	Let $X$ be a topological space and define $\iota,\jota : X \to X \times I$ by 
	\begin{equation*}
		\iota(x) := (x,0) \qquad \text{and} \qquad \jota(x) := (x,1).
	\end{equation*}
	Then $H_n(\iota) = H_n(\jota)$ for all $n \in \omega$.
\end{proposition}

\begin{theorem}[The Homotopy Axiom]
	Let $f,g \in \mathsf{Top}(X,Y)$ be freely homotopic. Then $H_n(f) = H_n(g)$ for all $n \in \omega$.
\end{theorem}

\begin{proof}
	Using the notation and the result from proposition \ref{prop:inclusions}, we get that
	\begin{align*}
		H_n(f) = H_n(F \circ \iota) = H_n(F) \circ H_n(\iota) = H_n(F) \circ H_n(\jota) = H_n(F \circ \jota) = H_n(g).
	\end{align*}
\end{proof}

